ch2o_compcertc_lp64.v
@@ -1,0 +1,162 @@
+From ch2o_compcert Require Export ch2o_safety compcertc_safety.
+From ch2o Require Export stringmap types expressions statements architectures state.
+From compcert Require Export Csyntax Ctypes Globalenvs.
+
+Section Program.
+
+Local Open Scope string_scope.
+
+(* We prove soundness for LP64 architectures. *)
+
+Definition A: architecture := {|
+  arch_sizes := architectures.lp64;
+  arch_big_endian := false;
+  arch_char_signedness := integer_coding.Signed;
+  arch_alloc_can_fail := false
+|}.
+Notation K := (arch_rank A).
+
+Context (Γ: types.env K) (δ: funenv K) (p: Csyntax.program).
+
+Inductive expr_equiv: expressions.expr K → Csyntax.expr → Prop :=
+| expr_equiv_val_int z:
+  int_typed z (sintT: int_type K) → (* TODO: Require the CH2O program to be well-typed instead? *)
+  expr_equiv (EVal ∅ (inr (intV{sintT} z))) (Eval (Vint (Int.repr z)) (Tint I32 Signed noattr)).
+
+Inductive stmt_equiv: stmt K → statement → Prop :=
+| stmt_equiv_Return e ė:
+  expr_equiv e ė →
+  stmt_equiv (SReturn e) (Sreturn (Some ė))
+.
+
+Inductive program_equiv: Prop :=
+| program_equiv_intro s ṡ m b:
+  stringmap_lookup "main" δ = Some s →
+  Genv.init_mem p = Some m →
+  let ge := globalenv p in
+  Genv.find_symbol ge p.(prog_main) = Some b →
+  let f := {|
+    fn_return:=type_int32s;
+    fn_callconv:=AST.cc_default;
+    fn_params:=nil;
+    fn_vars:=nil;
+    fn_body:=ṡ
+  |} in
+  Genv.find_funct_ptr ge b = Some (Internal f) →
+  stmt_equiv s ṡ →
+  program_equiv.
+
+Theorem soundness Q:
+  program_equiv →
+  ch2o_safe_program Γ δ Q →
+  compcertc_safe_program Q p.
+Proof.
+intros Hequiv Hch2o.
+destruct Hequiv.
+econstructor. { econstructor; try eassumption. reflexivity. }
+intro; intros.
+(* Callstate *)
+inversion H4; clear H4; subst. {
+  right.
+  eexists.
+  eexists.
+  right.
+  eapply step_internal_function. {
+    constructor.
+  } {
+    constructor.
+  } {
+    constructor.
+  }    
+}
+inversion H5; clear H5; subst; inversion H4; clear H4; subst.
+clear H1 H2 H12 H14.
+inversion H13; clear H13; subst.
+simpl in H6.
+(* Executing the body *)
+inversion H3; clear H3; subst.
+inversion H6; clear H6; subst. {
+  right.
+  eexists.
+  eexists.
+  right.
+  constructor.
+}
+inversion H2; clear H2; subst; inversion H4; clear H4; subst.
+(* Returning *)
+inversion H1; clear H1; subst.
+inversion H3; clear H3; subst. {
+  right.
+  eexists.
+  eexists.
+  right.
+  constructor.
+  - reflexivity.
+  - reflexivity.
+}
+inversion H1; clear H1; subst; inversion H3; clear H3; subst; try (inversion H12; clear H12; subst; try discriminate).
+{ subst; inversion H11. }
+{ subst; inversion H11. }
+{ inversion H11; clear H11; subst; try discriminate.
+  subst.
+  elim H12.
+  constructor. }
+(* Final state *)
+assert (Cop.sem_cast (Vint (Int.repr z)) (Tint I32 Signed noattr) type_int32s m2 = Some (Vint (Int.repr z))). {
+  unfold Cop.sem_cast in H4.
+  simpl in H4.
+  destruct Archi.ptr64; reflexivity. (* TODO: We may at some point need to make an assumption about this. *)
+}
+rewrite H1 in H4.
+simpl in H4.
+inversion H4; clear H4; subst. 2:{
+  inversion H3; clear H3; subst; inversion H4.
+}
+left.
+constructor.
+rewrite Int.signed_repr. 2:{
+  inversion H2.
+  unfold int_lower in H3; simpl in H3.
+  unfold int_upper in H4; simpl in H4.
+  unfold Int.min_signed; unfold Int.max_signed.
+  unfold Int.half_modulus.
+  unfold Int.modulus.
+  unfold Int.wordsize.
+  unfold Wordsize_32.wordsize.
+  split.
+  - apply H3.
+  - simpl. lia.
+}
+(* Proving Q z *)
+destruct (Hch2o (state.State [] (Return "main" (intV{sintT} z)) ∅)). 2:{
+  inversion H3; assumption.
+} 2:{
+  destruct H3.
+  inversion H3.
+}
+(* Showing a CH2O execution *)
+(* Calling main *)
+eapply rtc_l. {
+  econstructor.
+  - apply H.
+  - constructor.
+  - reflexivity.
+}
+simpl.
+(* Starting executing ret *)
+eapply rtc_l. {
+  apply cstep_expr with (E:=CReturnE: statements.esctx_item K) (e:=(# intV{sintT} z: expressions.expr K)%E).
+}
+(* Finishing executing ret *)
+eapply rtc_l. {
+  constructor.
+}
+rewrite mem_unlock_empty.
+(* Returning from main *)
+eapply rtc_l. {
+  constructor.
+}
+apply rtc_refl.
+Qed.
+
+End Program.
